coq/EqDec.v
@@ -59,6 +59,9 @@ Proof.
   - congruence.
 Qed.
 
+Lemma neq_dec {A} {EQ: Eqdec A}:
+  exists x, forall a b, a <> b -> eq_dec a b = right x.
+
 Lemma beq_dec_refl {A} {EQ: EqDec A}: forall a, beq_dec a a = true.
 Proof.
   intros.
